Revert hands-on tasks

Imp/Expr/Optimize.lean
@@ -3,53 +3,29 @@ import Imp.Expr.Eval
 
 namespace Imp.Expr
 
-def optOp : BinOp → Expr → Expr → Expr
-  | bop, .const i, .const i' =>
-    if let some v := bop.apply i i' then .const v
-    else .op bop (.const i) (.const i')
-  | .plus, .const 0, e2 => e2
-  | bop, e1, e2 => .op bop e1 e2
-
 /--
 Optimizes an expression by folding constants.
 -/
 def optimize : Expr → Expr
   | .const i => .const i
   | .var x => .var x
-  | .unop uop e =>
-    match optimize e with
-    | .const i =>
-      if let some v := uop.apply i then .const v
-      else .unop uop (.const i)
-    | e' => .unop uop e'
   | .op bop e1 e2 =>
-    .optOp bop e1.optimize e2.optimize
+    match optimize e1, optimize e2 with
+    | .const i, .const i' =>
+      if let some v := bop.apply i i' then .const v
+      else .op bop (.const i) (.const i')
+    | e1', e2' => .op bop e1' e2'
 
-@[simp]
-theorem BinOp.apply_plus_0 (v : Value) :  BinOp.plus.apply (0#32) v = v  :=
-  by simp [BinOp.apply]
-
-@[simp]
-theorem optOp_ok (bop : BinOp) (e1 e2 : Expr) : (optOp bop e1 e2).eval σ = (op bop e1 e2).eval σ  := by
-  unfold optOp
-  split
-  · split
-    · simp [eval, *]
-    · simp [eval, *]
-  · simp [eval, *]
-  · simp [eval, *]
-
+/--
+Optimization doesn't change the meaning of any expression
+-/
 theorem optimize_ok (e : Expr) : e.eval σ = e.optimize.eval σ := by
-  induction e
-  case unop uop e ih =>
-    unfold optimize
+  induction e <;> simp [optimize]
+  case op bop e1 e2 ih1 ih2 =>
     split <;> simp [eval, *]
     split
     · simp [eval, *]
     · simp [eval]
-  case op bop e1 e2 ih1 ih2 =>
-    unfold optimize
-    simp [eval, *]
 
 /--
 Optimization doesn't change the meaning of any expression
