Imp/Expr/Basic.lean
@@ -1,9 +1,5 @@
 namespace Imp
 
-inductive UnOp where
-  | neg | not
-deriving Repr, DecidableEq
-
 /-- Binary operators -/
 inductive BinOp where
   | plus | minus | times | div
@@ -17,7 +13,6 @@ deriving Repr, DecidableEq
 inductive Expr where
   | const (i : BitVec 32)
   | var (name : String)
-  | unop (op : UnOp) (e : Expr)
   | op (op : BinOp) (e1 e2 : Expr)
 deriving Repr, DecidableEq
 
